fairness/examples/ticketlock/fair_lock_lm.v
@@ -54,11 +54,13 @@ Section FairLockLM.
 
   Let LMF := LM_Fair (LF := LF).
 
-  Let lift_prop1 (P: R -> fmstate M -> Prop): 
+  Let lift_prop1 (P1 P2: R -> fmstate M -> Prop): 
     fmrole LMF -> lm_ls LM -> Prop := 
         fun g δ => let '(asG ρ) := g in
+                 let st := ls_under δ in
                  g ∈ dom $ ls_tmap δ /\
-                 P ρ (ls_under δ). 
+                 (P1 ρ st /\ (role_enabled_model ρ st \/ ¬ role_enabled_model g δ) \/
+                  P2 ρ st /\ ¬ role_enabled_model ρ st /\ role_enabled_model g δ). 
 
   (*TODO: move *)
   Lemma gset_singleton_dec `{Countable K}:
@@ -80,9 +82,9 @@ Section FairLockLM.
     rewrite union_empty_r_L. left. eauto.
   Qed. 
 
-  Instance lift_prop1_dec P
-    (DECP: forall ρ st, Decision (P ρ st)):
-    forall g δ, Decision (lift_prop1 P g δ).
+  Instance lift_prop1_dec P1 P2
+    (DECP1: forall ρ st, Decision (P1 ρ st)) (DECP2: forall ρ st, Decision (P2 ρ st)):
+    forall g δ, Decision (lift_prop1 P1 P2 g δ).
   Proof. 
     intros [g] δ. rewrite /lift_prop1.
     solve_decision. 
@@ -97,96 +99,236 @@ Section FairLockLM.
     all: right; lia.
   Qed.
 
-  Let active_st '(asG ρ) δ :=
-        ls_tmap δ !! (asG ρ) = Some {[ ρ ]} /\
-        lift_prop1 active_st (asG ρ) δ.
-
-  Let disabled_st '(asG ρ) (δ: lm_ls LM) :=
-        ls_tmap δ !! (asG ρ) = Some ∅ /\
-        lift_prop1 disabled_st (asG ρ) δ.
-
   Instance FLP_LMF: FairLockPredicates LMF.
   refine {| 
-      can_lock_st := lift_prop1 can_lock_st;
-      has_lock_st := lift_prop1 has_lock_st;
-      fair_lock.active_st := active_st;
-      fair_lock.disabled_st := disabled_st;
+      does_lock := lift_prop1 does_lock does_unlock;
+      does_unlock := lift_prop1 does_unlock does_lock;
       is_unused := fun g δ => g ∉ dom $ ls_tmap δ;
     |}.
-  - intros [?] ?. solve_decision.
-  - intros [?] ?. rewrite /disabled_st. solve_decision.
   Defined.
 
   Definition lift_prop2 (P: fmrole M -> fmstate M -> fmstate M -> Prop):
-    fmrole LMF -> lm_ls LM -> lm_ls LM -> Prop := 
+    fmrole LMF -> lm_ls LM -> lm_ls LM -> Prop :=
         fun '(asG ρ) δ1 δ2 =>
             ls_tmap δ1 !! (asG ρ) = Some ∅ /\
             ls_tmap δ2 = <[ asG ρ := {[ ρ ]} ]> (ls_tmap δ1) /\
             ls_fuel δ2 = <[ ρ := lm_fl LM (ls_under δ2) ]> (ls_fuel δ1) /\
             P ρ (ls_under δ1) (ls_under δ2).
 
-  Definition allows_unlock := lift_prop2 allows_unlock. 
-  Definition allows_lock := lift_prop2 allows_lock.
+  Definition au_impl := lift_prop2 au_impl. 
+  Definition al_impl := lift_prop2 al_impl. 
 
   Instance lift_prop2_dec P
     (DECP: forall ρ st1 st2, Decision (P ρ st1 st2)):
     forall g δ1 δ2, Decision (lift_prop2 P g δ1 δ2).
   Proof.
     intros [g] δ1 δ2. rewrite /lift_prop2.
-    solve_decision. 
+    solve_decision.
   Qed.
 
   Instance allows_lock_ex_dec:
-    forall δ g, Decision (∃ δ', allows_lock g δ δ'). 
+    forall δ g, Decision (∃ δ', al_impl g δ δ').
   Proof using LSI_DEC FLP FL.
-    clear MAP_RESTR UNUSED_NOT_DOM. 
+    clear MAP_RESTR UNUSED_NOT_DOM.
     intros δ [ρ]. simpl.
-    eapply Decision_iff_impl. 
-    { setoid_rewrite allows_lock_impl_spec.
-      reflexivity. }
+    eapply Decision_iff_impl.
+    { setoid_rewrite allows_lock_impl_spec. reflexivity. }
     destruct (decide (ls_tmap δ !! asG ρ = Some ∅ /\
-                      can_lock_st ρ δ ∧ fair_lock.disabled_st ρ δ)). 
+                      does_lock ρ δ ∧ disabled_st ρ δ)).
     2: { right. set_solver. }
     destruct (let st' := (allow_lock_impl ρ δ) in build_ls_ext st' (<[asG ρ:={[ρ]}]> (ls_tmap δ)) (<[ρ:=lm_fl LM st']> (ls_fuel δ)) (H0 := LSI_DEC)).
     { left. destruct e as [δ2 (?&?&?)]. exists δ2.
       repeat split; try by apply a || eauto.
       congruence. }
     right. intros (?&?&?&?&?&?&?).
-    destruct n. eexists. repeat split; eauto. congruence. 
-  Qed. 
+    destruct n. eexists. repeat split; eauto. congruence.
+  Qed.
 
   Instance allows_unlock_ex_dec:
-    forall δ g, Decision (∃ δ', allows_unlock g δ δ'). 
+    forall δ g, Decision (∃ δ', au_impl g δ δ').
   Proof using LSI_DEC FLP FL.
-    clear MAP_RESTR UNUSED_NOT_DOM. 
+    clear MAP_RESTR UNUSED_NOT_DOM.
     intros δ [ρ]. simpl.
-    eapply Decision_iff_impl. 
+    eapply Decision_iff_impl.
     { setoid_rewrite allows_unlock_impl_spec. reflexivity. }
     destruct (decide (ls_tmap δ !! asG ρ = Some ∅ /\
-                      has_lock_st ρ δ ∧ fair_lock.disabled_st ρ δ)). 
+                      does_unlock ρ δ ∧ disabled_st ρ δ)).
     2: { right. set_solver. }
     destruct (let st' := (allow_unlock_impl ρ δ) in build_ls_ext st' (<[asG ρ:={[ρ]}]> (ls_tmap δ)) (<[ρ:=lm_fl LM st']> (ls_fuel δ)) (H0 := LSI_DEC)).
     { left. destruct e as [δ2 (?&?&?)]. exists δ2.
       repeat split; try by apply a || eauto.
       congruence. }
     right. intros (?&?&?&?&?&?&?).
-    destruct n. eexists. repeat split; eauto. congruence. 
+    destruct n. eexists. repeat split; eauto. congruence.
   Qed.
 
   Let tl_active_exts (δ: fmstate LMF): gset fl_EI := 
       set_map (flU (M := LMF)) 
-          (filter (fun g => exists δ', allows_unlock g δ δ') (dom (ls_tmap δ)))
+          (filter (fun g => exists δ', au_impl g δ δ') (dom (ls_tmap δ)))
       ∪
       set_map (flL (M := LMF)) 
-          (filter (fun g => exists δ', allows_lock g δ δ') (dom (ls_tmap δ))).
+          (filter (fun g => exists δ', al_impl g δ δ') (dom (ls_tmap δ))).
     
 
-  Instance FLE_LMF: FairLockExt LMF.
+  (* TODO: move*)
+  From trillium.fairness Require Import partial_ownership.
+  Hypothesis LSI_LIFTS_STEP: forall (δ1: lm_ls LM) ρ st2,
+      fmtrans _ (ls_under δ1) (Some ρ) st2 ->
+      LSI st2 (ls_tmap δ1) (ls_fuel δ1).
+  Hypothesis LSI_FUEL_INDEP: LSI_fuel_independent (LSI := LSI). 
+  Hypothesis M_STRONG_LR: FM_strong_lr M.
+  Hypothesis STEP_NO_EN: forall st1 ρ st2,
+      fmtrans M st1 (Some ρ) st2 ->
+      live_roles _ st2 ⊆ live_roles _ st1. 
+ Hypothesis DROP_PRES_LSI: forall st rem, fuel_drop_preserves_LSI st rem (LSI := LSI). 
+
+  (* TODO: move? generalize? *)
+  Lemma enabled_group_singleton ρ δ:
+    role_enabled_model ((asG ρ): fmrole LMF) δ <->
+    ρ ∈ dom (ls_mapping δ).
+  Proof.
+    split; intros EN.
+    { red in EN. apply LM_live_roles_strong in EN as [? STEP].
+      red in STEP. destruct STEP as (ℓ & STEP & MATCH).
+      destruct ℓ; simpl in MATCH; subst; simpl in STEP.
+      - destruct STEP as (STEP & MAP & _).
+        apply MAP_RESTR in MAP. inversion MAP. subst.
+        apply ls_mapping_dom. eapply fm_live_spec; eauto.
+      - destruct STEP as ([ρ_ MAP] & DECR & NINCR & _).
+        pose proof MAP as MAP'%MAP_RESTR. inversion MAP'. subst ρ_. clear MAP'.
+        eapply elem_of_dom. eauto.
+      - done. }
+    apply elem_of_dom in EN as [g MAP].
+    pose proof MAP as MAP'%MAP_RESTR. subst g.
+    destruct (decide (ρ ∈ live_roles _ (ls_under δ))) as [EN | DIS].
+    - red. apply M_STRONG_LR in EN as [st2 STEP].
+      pose proof MAP as [f F]%mk_is_Some%ls_same_doms'. 
+      assert (exists δ': lm_ls LM, ls_under δ' = st2 /\ ls_tmap δ' = ls_tmap δ /\ ls_fuel δ' = <[ ρ := min (lm_fl LM st2) f ]> (ls_fuel δ)) as [δ' (ST' & TM' & F')]. 
+      {
+        unshelve eexists {| ls_under := st2 |}.
+        7: repeat split; reflexivity. 
+        3: by apply δ. 
+        { etrans; [eapply STEP_NO_EN; eauto| ].
+          rewrite dom_insert_L. pose proof (ls_fuel_dom δ). set_solver. }
+        2: { apply LSI_FUEL_INDEP with (F := ls_fuel δ). 
+             eapply LSI_LIFTS_STEP; eauto. }
+        intros. rewrite -(ls_tmap_fuel_same_doms δ).
+        apply mk_is_Some, ls_same_doms', elem_of_dom in MAP. 
+        rewrite dom_insert_L. set_solver. } 
+      (* rewrite ST' in *.  *)
+      (* subst.  *)
+      apply fm_live_spec with (s' := δ'). simpl.
+      exists (Take_step ρ (asG ρ)). split; [| done]. simpl.
+      Set Printing Coercions.
+      repeat split; eauto; try congruence. 
+      + red. rewrite !F'. intros ρ' DOM DOM' DEC.
+        inversion DEC; subst.
+        * symmetry in Hsametid. apply MAP_RESTR in Hsametid. congruence.
+        * destruct Hneqtid. f_equal.
+          rewrite /ls_mapping. congruence.
+      + red. rewrite !F'. intros.
+        apply elem_of_dom in H as [? F2]. 
+        destruct (decide (ρ' = ρ)) as [-> | NEQ].
+        2: { left. rewrite lookup_insert_ne; [| done].
+             rewrite F2. simpl. lia. }
+        left. rewrite lookup_insert F. simpl. lia. 
+      + rewrite !F' ST'. simpl. intros.
+        rewrite lookup_insert. simpl. lia. 
+      + intros ?. rewrite F' dom_insert_L.
+        apply mk_is_Some, elem_of_dom in F. set_solver. 
+      + rewrite F' dom_insert_L.
+        apply mk_is_Some, elem_of_dom in F. set_solver. 
+    - red.
+      assert (exists δ': lm_ls LM, ls_under δ' = ls_under δ /\ ls_tmap δ' = (fun rs => rs ∖ {[ ρ ]}) <$> ls_tmap δ /\ ls_fuel δ' = delete ρ (ls_fuel δ)) as [δ' (ST' & TM' & F')]. 
+      { unshelve eexists (MkLiveState _ _ _ _ _ _ _).
+        8: repeat split; simpl; reflexivity.
+        - pose proof (ls_fuel_dom δ). set_solver. 
+        - intros. apply mapped_roles_dom_fuels_gen. 
+          rewrite groups_map_difference. 
+          rewrite dom_delete_L. f_equal.
+          apply mapped_roles_dom_fuels_gen. apply δ. 
+        - red. intros * NEQ (?&<-&TM1)%lookup_fmap_Some (?&<-&TM2)%lookup_fmap_Some.
+          eapply disjoint_subseteq.
+          { apply _. }
+          3: { eapply ls_tmap_disj; eauto. }
+          all: set_solver. 
+        - eapply DROP_PRES_LSI, δ. }
+      apply fm_live_spec with (s' := δ'). simpl.
+      simpl. exists (Silent_step (asG ρ)). split; [| done].
+      simpl. repeat split; eauto.
+      + red. rewrite !F'. simpl. intros ρ' DOM1 DOM2 DECR.
+        apply dom_delete, elem_of_difference in DOM2.
+        rewrite not_elem_of_singleton in DOM2. apply proj2 in DOM2. 
+        inversion DECR.
+        * subst. symmetry in Hsametid. apply MAP_RESTR in Hsametid. congruence.
+        * subst. destruct Hissome as [g MAP'].
+          pose proof MAP' as ?%MAP_RESTR. subst.
+          rewrite -ls_same_doms elem_of_dom in DOM1.
+          destruct DOM1 as [? MAP1].
+          pose proof MAP1 as ?%MAP_RESTR. subst. congruence.
+      + red. rewrite !ST' !F'. intros ρ' DOM'. 
+        destruct (decide (ρ' = ρ)) as [-> | ?].
+        * repeat right. set_solver.
+        * left. apply elem_of_dom in DOM' as [? F1].
+          rewrite lookup_delete_ne; [| done].
+          rewrite F1. simpl. lia.
+      + rewrite F'. set_solver.
+  Qed. 
+
+  Lemma disabled_group_singleton ρ δ:
+    ¬ role_enabled_model ((asG ρ): fmrole LMF) δ <-> ρ ∉ dom (ls_mapping δ).
+  Proof. 
+    apply not_iff_compat. apply enabled_group_singleton.
+  Qed. 
+
+  Lemma disabled_group_disabled_role ρ δ:
+    ¬ role_enabled_model ((asG ρ): fmrole LMF) δ -> ¬ role_enabled_model ρ (ls_under δ). 
+  Proof.
+    by intros ? ?%ls_mapping_dom%enabled_group_singleton.
+  Qed.
+
+  Instance FLE_LMF: @FairLockExt LMF FLP_LMF.
   refine {|
-      fair_lock.allows_unlock := allows_unlock;
-      fair_lock.allows_lock := allows_lock;
+      fair_lock.au_impl := au_impl;
+      fair_lock.al_impl := al_impl;
       fair_lock.fl_active_exts := tl_active_exts;
-    |}. 
+    |}.
+  { simpl. intros [ρ] * AU. red in AU. simpl in AU.
+    destruct AU as (TM0 & TM' & FUEL' & AU).
+    apply au_impl_spec in AU. 
+    red. repeat split.
+    - by apply elem_of_dom.
+    - left. split.
+      + apply AU.
+      + right. apply LM_map_empty_notlive. by left.
+    - apply LM_map_empty_notlive. by left.
+    - rewrite TM'. set_solver.
+    - left. split.
+      + apply AU.
+      + left. apply AU.
+    - apply enabled_group_singleton.
+      eapply mim_in_2 with (v := asG ρ); eauto. 
+      { apply (ls_mapping_tmap_corr st2). }
+      rewrite TM'. rewrite lookup_insert. set_solver. }
+  (* TODO: refactor *)
+  { simpl. intros [ρ] * AU. red in AU. simpl in AU.
+    destruct AU as (TM0 & TM' & FUEL' & AU).
+    apply al_impl_spec in AU. 
+    red. repeat split.
+    - by apply elem_of_dom.
+    - left. split.
+      + apply AU. 
+      + right. apply LM_map_empty_notlive. by left.
+    - apply LM_map_empty_notlive. by left.
+    - rewrite TM'. set_solver.
+    - left. split.
+      + apply AU.
+      + left. apply AU.
+    - apply enabled_group_singleton.
+      eapply mim_in_2 with (v := asG ρ); eauto. 
+      { apply (ls_mapping_tmap_corr st2). }
+      rewrite TM'. rewrite lookup_insert. set_solver. }
+  
   intros. simpl.
   unfold tl_active_exts.
   rewrite elem_of_union.
@@ -204,7 +346,7 @@ Section FairLockLM.
        intros [-> [? AU]]. do 2 red in AU.
        destruct g. apply elem_of_dom.
        by rewrite (proj1 AU). }
-  destruct ι; set_solver. 
+  destruct ι; try set_solver. 
   Defined.
 
   Lemma LM_EM_EXT_KEEPS: ext_keeps_asg
@@ -242,14 +384,12 @@ Section FairLockLM.
                 (@ETs _ (FL_EM FLE)) (proj_ext ι) (ls_under δ1) (ls_under δ2).
   Proof. 
     intros ? ι ? STEP. 
-    destruct ι as [[ρ]| [ρ]]; simpl in *; apply STEP.
+    destruct ι as [[ρ]| [ρ]]; simpl in *; set_solver. 
   Qed. 
-
-
   
   (* TODO: move, generalize *)
   Lemma upto_state_lookup_unfold2 i δ
-    (lmtr: mtrace (@ext_model_FM LMF (@FL_EM LMF FLE_LMF)))
+    (lmtr: mtrace (@ext_model_FM LMF (@FL_EM LMF _ FLE_LMF)))
     (mtr: trace M (option ext_role))
     (UPTO: upto_stutter_eauxtr proj_ext lmtr mtr)
     (ITH : lmtr S!! i = Some δ):
@@ -269,7 +409,7 @@ Section FairLockLM.
 
   (* TODO: move, generalize *)
   Lemma upto_state_lookup_unfold1 i' st
-    (lmtr: mtrace (@ext_model_FM LMF (@FL_EM LMF FLE_LMF)))
+    (lmtr: mtrace (@ext_model_FM LMF (@FL_EM LMF _ FLE_LMF)))
     (mtr: trace M (option ext_role))
     (UPTO: upto_stutter_eauxtr proj_ext lmtr mtr)
     (ITH : mtr S!! i' = Some st):
@@ -287,66 +427,81 @@ Section FairLockLM.
     eapply upto_stutter_trfirst; eauto.
   Qed. 
   
-  Definition others_or_burn ρ' :=
+  Definition others_or_burn ρ' (fl_ctr: G -> @EI _ (FL_EM FLE_LMF)) :=
     (λ δ1 oℓ δ2,
        match oℓ with
        | Some (inl g) => next_TS_role δ1 g δ2 ≠ Some ρ'
-       | _ => other_proj (asG ρ') oℓ
-       end). 
+       | Some (inr (env e)) => e ≠ fl_ctr (asG ρ')
+       | None => True
+       end).
 
-  Lemma others_or_burn_keep_inner_prop P (ρ': fmrole M)
-    (KEPT: label_kept_state
-        (λ st : ext_model_FM, P st)
-        (other_proj ρ')):
-    label_kept_state_gen
-    (λ st' : fmstate (@ext_model_FM _ (FL_EM FLE_LMF)),
-       P st')
-    (others_or_burn ρ').
-  Proof.
-    red. intros. simpl in STEP. inversion STEP; subst.
-    - simpl in STEP0. unfold_LMF_trans STEP0.
-      + eapply KEPT. 
-        { apply P1. }
-        2: { simpl. left. simpl. apply STEP1. }                   
-        red. simpl. intros ->. congruence. 
-      + repeat apply proj2 in STEP1. congruence.
-    - destruct ι; simpl in REL; red in REL.
-      + destruct ρ as [ρ]. 
-        eapply KEPT. 
-        { apply P1. }
-        2: { simpl. right. Unshelve. 2: exact (flU ρ).
-             apply REL. }
-        red. simpl.
-        intros ->. simpl in PSTEP. congruence.
-      + destruct ρ as [ρ]. 
-        eapply KEPT.
-        { apply P1. }
-        2: { simpl. right. Unshelve. 2: exact (flL ρ).
-             apply REL. }
-        red. simpl.
-        intros ->. simpl in PSTEP. congruence.
-  Qed.
+  Instance oob_dec: forall ρ fl_ctr δ1 ℓ δ2, Decision (others_or_burn ρ fl_ctr δ1 ℓ δ2). 
+  Proof. 
+    rewrite /others_or_burn. destruct ℓ as [[|]|]; try solve_decision.
+    intros. destruct e; solve_decision. 
+  Qed. 
 
   Lemma others_or_burn_keep_lock ρ':
     label_kept_state_gen
     (λ st' : fmstate (@ext_model_FM _ (FL_EM FLE_LMF)),
-       has_lock_st ρ' (ls_under st') ∧ fair_lock.disabled_st ρ' (ls_under st'))
-    (others_or_burn ρ').
+       does_unlock ρ' (ls_under st') ∧ fair_lock.disabled_st ρ' (ls_under st'))
+    (others_or_burn ρ' (flU: @fmrole LMF -> @EI _ (FL_EM FLE_LMF))).
   Proof.
-    forward eapply others_or_burn_keep_inner_prop. 
-    { apply (step_keeps_lock_dis ρ'). }
-    done. 
+    red. intros. simpl in STEP. inversion STEP; subst.
+    - simpl in STEP0. unfold_LMF_trans STEP0.
+      + eapply step_keeps_unlock_dis. 
+        { apply P1. }
+        2: { simpl. left. simpl. apply STEP1. }                   
+        red. simpl. congruence. 
+      + repeat apply proj2 in STEP1. congruence.
+    - simpl in PSTEP.      
+      destruct ι; simpl in REL; red in REL.
+      + destruct ρ as [ρ]. 
+        eapply step_keeps_unlock_dis.
+        { apply P1. }
+        2: { simpl. right. Unshelve. 2: exact (flU ρ).
+             apply REL. }
+        red. simpl.
+        congruence. 
+      + destruct ρ as [ρ]. 
+        eapply step_keeps_unlock_dis.
+        { apply P1. }
+        2: { simpl. right. Unshelve. 2: exact (flL ρ).
+             apply REL. }
+        red. simpl.
+        congruence.
   Qed. 
+ 
 
   Lemma others_or_burn_keep_can_lock ρ':
     label_kept_state_gen
     (λ st' : fmstate (@ext_model_FM _ (FL_EM FLE_LMF)),
-       can_lock_st ρ' (ls_under st') ∧ fair_lock.disabled_st ρ' (ls_under st'))
-    (others_or_burn ρ').
+       does_lock ρ' (ls_under st') ∧ fair_lock.disabled_st ρ' (ls_under st'))
+    (others_or_burn ρ' (flL: @fmrole LMF -> @EI _ (FL_EM FLE_LMF))).
   Proof.
-    forward eapply others_or_burn_keep_inner_prop. 
-    { apply (step_keeps_can_lock_dis ρ'). }
-    done. 
+    red. intros. simpl in STEP. inversion STEP; subst.
+    - simpl in STEP0. unfold_LMF_trans STEP0.
+      + eapply step_keeps_lock_dis. 
+        { apply P1. }
+        2: { simpl. left. simpl. apply STEP1. }                   
+        red. simpl. congruence. 
+      + repeat apply proj2 in STEP1. congruence.
+    - simpl in PSTEP.      
+      destruct ι; simpl in REL; red in REL.
+      + destruct ρ as [ρ]. 
+        eapply step_keeps_lock_dis.
+        { apply P1. }
+        2: { simpl. right. Unshelve. 2: exact (flU ρ).
+             apply REL. }
+        red. simpl.
+        congruence. 
+      + destruct ρ as [ρ]. 
+        eapply step_keeps_lock_dis.
+        { apply P1. }
+        2: { simpl. right. Unshelve. 2: exact (flL ρ).
+             apply REL. }
+        red. simpl.
+        congruence.
   Qed. 
 
   (* TODO: move *)
@@ -392,7 +547,7 @@ Section FairLockLM.
     (ρ' : fmrole M)
   (st' : fmstate M)
   (VALID: mtrace_valid lmtr)
-  (HAS_LOCK : has_lock_st ρ' st')
+  (HAS_LOCK : does_unlock ρ' st')
   (DIS : fair_lock.disabled_st ρ' st')
   (FAIR: ∀ g, fair_by_group (ELM_ALM LM_EM_EXT_KEEPS) g lmtr)
   (i : nat)
@@ -401,14 +556,14 @@ Section FairLockLM.
   (ITH' : st' = ls_under (trfirst lmtr_i))
     :
 (exists i' st', i <= i' /\
-                        lmtr S!! i' = Some st' /\ has_lock_st ρ' st' /\
+                        lmtr S!! i' = Some st' /\ does_unlock ρ' st' /\
                         (* ¬ role_enabled_model ρ' st' /\ *)
                         ρ' ∉ dom (ls_mapping st') /\
                         ∀ (k : nat) (st' : fmstate ext_model_FM),
                           0 <= k <= i' - i
                           → lmtr_i S!! k = Some st'
                           → (λ δ: lm_ls LM,
-                                has_lock_st ρ' (ls_under δ)
+                                does_unlock ρ' (ls_under δ)
                                 ∧ fair_lock.disabled_st ρ' (ls_under δ)) st').
   Proof.
     assert (lmtr S!! i = Some (trfirst lmtr_i)) as ITH.
@@ -463,30 +618,29 @@ Section FairLockLM.
           0 <= k <= m
           → lmtr_i S!! k = Some st'
           → (λ δ : LiveState G M LSI,
-                has_lock_st ρ' (ls_under δ)
+                does_unlock ρ' (ls_under δ)
                 ∧ fair_lock.disabled_st ρ' (ls_under δ)) st') as KEEP.
     { eapply steps_keep_state_gen.
       { eauto. }
       { eexists. split; eauto. rewrite state_lookup_0. reflexivity. }
       { apply others_or_burn_keep_lock. }
-      { intros * [_ ?] KTH.
-        destruct oℓ'; [| done]. simpl.
-        pose proof KTH as STEP. eapply trace_valid_steps' in STEP; [| eauto].
-        simpl in STEP.
-        destruct f as [| [ι]].
-        - intros EQ. specialize (MIN k). specialize_full MIN; [| lia].
-          do 2 eexists. split; [done| ].
-          red. right. simpl. red. simpl. do 3 eexists. repeat split; eauto.
-        - intros EQ. specialize (MIN k). specialize_full MIN; [| lia].
-          simpl in EQ.
-          assert (ls_tmap st1 !! (asG ρ') = Some ∅) as NOρ.
-          { destruct ι; subst; inversion STEP; subst; simpl in REL; apply REL. }
-          do 2 eexists. split; [done| ].
-          left. intros (?& MAP)%elem_of_dom.
-          assert (x = asG ρ') as ->.
-          { by apply MAP_RESTR in MAP. }
-          eapply ls_mapping_tmap_corr in MAP as (?&?&?).
-          rewrite NOρ in H0. set_solver. }
+      intros * [_ ?] KTH.
+      destruct oℓ'; [| done]. simpl.
+      pose proof KTH as STEP. eapply trace_valid_steps' in STEP; [| eauto].
+      simpl in STEP.
+      destruct f as [| [ι]].
+      - intros EQ. specialize (MIN k). specialize_full MIN; [| lia].
+        do 2 eexists. split; [done| ].
+        red. right. simpl. red. simpl. do 3 eexists. repeat split; eauto.
+      - intros ->. specialize (MIN k). specialize_full MIN; [| lia].
+        assert (ls_tmap st1 !! (asG ρ') = Some ∅) as NOρ.
+        { inversion STEP; subst; simpl in REL; apply REL. }
+        do 2 eexists. split; [done| ].
+        left. intros (?& MAP)%elem_of_dom.
+        assert (x = asG ρ') as ->.
+        { by apply MAP_RESTR in MAP. }
+        eapply ls_mapping_tmap_corr in MAP as (?&?&?).
+        rewrite NOρ in H0. set_solver. 
     }
     
     clear HAS_LOCK DIS.
@@ -510,8 +664,208 @@ Section FairLockLM.
     { eauto. }
     intros ??.
     rewrite Nat.sub_add'. apply KEEP.
-  Qed. 
+  Qed.
 
+  Lemma has_lock_excl_lift: forall tl_st ρlg1 ρlg2,
+      does_unlock ρlg1 tl_st -> disabled_st ρlg1 tl_st ->
+      does_unlock ρlg2 tl_st -> disabled_st ρlg2 tl_st ->
+      ρlg1 = ρlg2.
+  Proof.
+    intros δ [ρ1] [ρ2].
+    simpl. intros [DOM1 UNLOCK1] DIS1 [DOM2 UNLOCK2] DIS2.
+    f_equal.
+    destruct UNLOCK1 as [UNLOCK1 | ?].
+    2: { red in DIS1. tauto. }  
+    destruct UNLOCK2 as [UNLOCK2 | ?].
+    2: { red in DIS2. tauto. }
+    destruct UNLOCK1 as [? [EN | DIS1']].
+    { apply ls_mapping_dom, enabled_group_singleton in EN. done. } 
+    destruct UNLOCK2 as [? [EN | DIS2']].
+    { apply ls_mapping_dom, enabled_group_singleton in EN. done. }
+    eapply has_lock_st_excl; eauto.
+    all: red; by intros ?%ls_mapping_dom%enabled_group_singleton.
+  Qed.     
+ 
+  (* TODO: refactor *)
+  Lemma does_lock_dis_kept:
+    ∀ ρ : fmrole LMF,
+    @label_kept_state (@ext_model_FM LMF (@FL_EM LMF _ FLE_LMF))
+      (λ st : fmstate (@ext_model_FM LMF (@FL_EM LMF _ FLE_LMF)),
+         @does_lock LMF FLP_LMF ρ st ∧ @fair_lock.disabled_st LMF FLP_LMF ρ st)
+      (fun oℓ => oℓ ≠ Some (inr (env ((@flL _ ρ): @EI _ (@FL_EM _ _ FLE_LMF)))))
+  .
+  Proof.
+    red. intros [ρ] δ oℓ δ' [LOCK DIS] OTHER STEP.
+    simpl in STEP. 
+    destruct LOCK as [DOM [LOCK | ]].
+    2: { red in DIS. tauto. }
+    pose proof DIS as DIS'%disabled_group_disabled_role. 
+    destruct LOCK as [LOCK [? | ?]]; [done| ]. 
+    assert (ρ ∉ dom (ls_mapping δ)) as ND. 
+    { by eapply disabled_group_singleton. }
+
+        
+    inversion STEP; subst.
+    -
+      assert (does_lock ρ (ls_under δ') /\ fair_lock.disabled_st ρ (ls_under δ') /\ ls_tmap δ' !! asG ρ = Some ∅) as (?&?&?).
+      { simpl in STEP0, LOCK, DIS.
+        simpl in OTHER.  destruct ρ0 as [ρ'].
+        unfold_LMF_trans STEP0.
+        2: { simpl in STEP1. pose proof STEP1 as SS. repeat apply proj2 in STEP1.
+            rewrite -STEP1. repeat split; try tauto.
+            apply unmapped_empty.
+            { intros ?. rewrite STEP1 in LOCK.
+              edestruct unused_does_lock_incompat; eauto. }
+            intros IN. 
+            pose proof SS.
+            do 3 apply proj2 in SS. apply proj1 in SS.
+            repeat rewrite -ls_same_doms in SS.
+            set_solver. }
+        forward eapply (step_keeps_lock_dis ρ (ls_under δ)).
+        { split; [apply LOCK | apply DIS']. }
+        2: { left. apply STEP1. }
+        { congruence. }
+        intros [??]. repeat split; eauto.
+        simpl in STEP1.
+        apply unmapped_empty.
+        { intros ?. edestruct unused_does_lock_incompat; eauto. }
+        intros IN.
+        repeat apply proj2 in STEP1. specialize (STEP1 ρ). specialize_full STEP1.
+        { apply elem_of_difference. repeat rewrite -ls_same_doms. split; [done| ].
+          intros IN'. done. }
+        apply elem_of_difference, proj1 in STEP1.
+        by destruct DIS'. }
+      
+      simpl. repeat split; eauto.
+      { by apply elem_of_dom. }
+      { left. split; [done| ]. right. apply LM_map_empty_notlive. by left. }
+      apply LM_map_empty_notlive. by left. 
+    - forward eapply (step_keeps_lock_dis ρ δ) as KEPT. 
+      { split; [apply LOCK| apply DIS']. }
+      2: { right. eapply PROJ_KEEP_EXT; eauto. }
+      { simpl. simpl in OTHER.
+        destruct ι; simpl; simpl in OTHER; red; destruct ρ0; congruence. }
+      intros. 
+      destruct ι; simpl in REL; red in REL.
+      + destruct ρ0 as [ρ']. assert (ρ' ≠ ρ).
+        { intros ->. repeat apply proj2 in REL. apply au_impl_spec in REL.
+          red in REL. eapply does_lock_unlock_incompat; eauto. apply REL. } 
+        simpl in *.
+        enough (ls_tmap δ' !! asG ρ = Some ∅).
+        { repeat split; eauto; try by apply KEPT.
+          { eapply elem_of_dom; eauto. }
+          { left. split; [apply KEPT| ]. right. apply LM_map_empty_notlive. by left. }
+          apply LM_map_empty_notlive. by left. }
+        
+        pose proof REL as REL_. 
+        apply proj2, proj1 in REL.
+        rewrite REL.
+        rewrite lookup_insert_ne; [| congruence].
+        apply unmapped_empty; try done.
+        intros ?. eapply unused_does_lock_incompat; eauto. 
+      + destruct ρ0 as [ρ']. assert (ρ' ≠ ρ) by set_solver. 
+        simpl in *.
+        enough (ls_tmap δ' !! asG ρ = Some ∅).
+        { repeat split; eauto; try by apply KEPT.
+          { eapply elem_of_dom; eauto. }
+          { left. split; [apply KEPT| ]. right. apply LM_map_empty_notlive. by left. }
+          apply LM_map_empty_notlive. by left. }
+        apply proj2, proj1 in REL. rewrite REL.
+        rewrite lookup_insert_ne; try congruence.
+        apply unmapped_empty; try done.
+        intros ?. eapply unused_does_lock_incompat; eauto. 
+  Qed.
+
+  (* TODO: refactor *)
+  Lemma does_unlock_dis_kept:
+    ∀ ρ : fmrole LMF,
+    @label_kept_state (@ext_model_FM LMF (@FL_EM LMF _ FLE_LMF))
+      (λ st : fmstate (@ext_model_FM LMF (@FL_EM LMF _ FLE_LMF)),
+         @does_unlock LMF FLP_LMF ρ st ∧ @fair_lock.disabled_st LMF FLP_LMF ρ st)
+      (fun oℓ => oℓ ≠ Some (inr (env ((@flU _ ρ): @EI _ (@FL_EM _ _ FLE_LMF)))))
+  .
+  Proof.
+    red. intros [ρ] δ oℓ δ' [LOCK DIS] OTHER STEP.
+    simpl in STEP. 
+    destruct LOCK as [DOM [LOCK | ]].
+    2: { red in DIS. tauto. }
+    pose proof DIS as DIS'%disabled_group_disabled_role. 
+    destruct LOCK as [LOCK [? | ?]]; [done| ]. 
+    assert (ρ ∉ dom (ls_mapping δ)) as ND. 
+    { by eapply disabled_group_singleton. }
+        
+    inversion STEP; subst.
+    -
+      assert (does_unlock ρ (ls_under δ') /\ fair_lock.disabled_st ρ (ls_under δ') /\ ls_tmap δ' !! asG ρ = Some ∅) as (?&?&?).
+      { simpl in STEP0, LOCK, DIS.
+        simpl in OTHER.  destruct ρ0 as [ρ'].
+        unfold_LMF_trans STEP0.
+        2: { simpl in STEP1. pose proof STEP1 as SS. repeat apply proj2 in STEP1.
+            rewrite -STEP1. repeat split; try tauto.
+            apply unmapped_empty.
+            { intros ?. rewrite STEP1 in LOCK.
+              edestruct unused_does_unlock_incompat; eauto. }
+            intros IN. 
+            pose proof SS.
+            do 3 apply proj2 in SS. apply proj1 in SS.
+            repeat rewrite -ls_same_doms in SS.
+            set_solver. }
+        forward eapply (step_keeps_unlock_dis ρ (ls_under δ)).
+        { split; [apply LOCK | apply DIS']. }
+        2: { left. apply STEP1. }
+        { congruence. }
+        intros [??]. repeat split; eauto.
+        simpl in STEP1.
+        apply unmapped_empty.
+        { intros ?. edestruct unused_does_unlock_incompat; eauto. }
+        intros IN.
+        repeat apply proj2 in STEP1. specialize (STEP1 ρ). specialize_full STEP1.
+        { apply elem_of_difference. repeat rewrite -ls_same_doms. split; [done| ].
+          intros IN'. done. }
+        apply elem_of_difference, proj1 in STEP1.
+        by destruct DIS'. }
+      
+      simpl. repeat split; eauto.
+      { by apply elem_of_dom. }
+      { left. split; [done| ]. right. apply LM_map_empty_notlive. by left. }
+      apply LM_map_empty_notlive. by left. 
+    - forward eapply (step_keeps_unlock_dis ρ δ) as KEPT. 
+      { split; [apply LOCK| apply DIS']. }
+      2: { right. eapply PROJ_KEEP_EXT; eauto. }
+      { simpl. simpl in OTHER.
+        destruct ι; simpl; simpl in OTHER; red; destruct ρ0; congruence. }
+      intros. 
+      destruct ι; simpl in REL; red in REL; cycle 1. 
+      + destruct ρ0 as [ρ']. assert (ρ' ≠ ρ).
+        { intros ->. repeat apply proj2 in REL. apply al_impl_spec in REL.
+          red in REL. eapply does_lock_unlock_incompat; eauto. apply REL. } 
+        simpl in *.
+        enough (ls_tmap δ' !! asG ρ = Some ∅).
+        { repeat split; eauto; try by apply KEPT.
+          { eapply elem_of_dom; eauto. }
+          { left. split; [apply KEPT| ]. right. apply LM_map_empty_notlive. by left. }
+          apply LM_map_empty_notlive. by left. }
+        
+        pose proof REL as REL_. 
+        apply proj2, proj1 in REL.
+        rewrite REL.
+        rewrite lookup_insert_ne; [| congruence].
+        apply unmapped_empty; try done.
+        intros ?. eapply unused_does_unlock_incompat; eauto. 
+      + destruct ρ0 as [ρ']. assert (ρ' ≠ ρ) by set_solver. 
+        simpl in *.
+        enough (ls_tmap δ' !! asG ρ = Some ∅).
+        { repeat split; eauto; try by apply KEPT.
+          { eapply elem_of_dom; eauto. }
+          { left. split; [apply KEPT| ]. right. apply LM_map_empty_notlive. by left. }
+          apply LM_map_empty_notlive. by left. }
+        apply proj2, proj1 in REL. rewrite REL.
+        rewrite lookup_insert_ne; try congruence.
+        apply unmapped_empty; try done.
+        intros ?. eapply unused_does_unlock_incompat; eauto. 
+  Qed.
+
+    
   Lemma ev_rel_inner (lmtr: elmftrace (ELM := FL_EM FLE_LMF))
     (mtr: trace M (option ext_role))
     (ρ : R)
@@ -521,7 +875,7 @@ Section FairLockLM.
     (EV_REL : eventual_release lmtr (asG ρ) 0):
   eventual_release mtr ρ 0.
   Proof.
-    red in EV_REL. 
+    (* red in EV_REL.  *)
     red. intros.
     forward eapply upto_state_lookup_unfold1 as (mtr_i' & i & lmtr_i & AFTERi & AFTERi' & UPTOi & ITH' & PREi); eauto.
     
@@ -535,28 +889,34 @@ Section FairLockLM.
 
     assert (ls_tmap δ_m !! asG ρ' = Some ∅) as DOMρ'.
     { apply unmapped_empty; auto. intros UN. 
-      edestruct unused_has_lock_incompat; eauto. } 
+      edestruct unused_does_unlock_incompat; eauto. } 
 
-    specialize (EV_REL (asG ρ')). specialize_full EV_REL.
+    forward eapply LM_map_empty_notlive as DISg'; [by left| ].
+    forward eapply eventual_release_strenghten2 with (ρ' := asG ρ': fmrole LMF).
+    { apply does_unlock_dis_kept. }
+    { apply has_lock_excl_lift. }    
+    { apply EV_REL. }
     { apply MTH. }
-    { simpl. split; eauto. eapply elem_of_dom. eauto. }
-    { split; eauto. 
-      red. split; [by eapply elem_of_dom| ]. 
-      eapply (BETWEEN (m - i)).
-      { lia. }
-      erewrite state_lookup_after; eauto.
-      rewrite -Nat.le_add_sub; eauto. } 
+    { simpl. split; [eapply elem_of_dom; eauto| tauto]. } 
+    { done. }
     { intros _. specialize (AFTER ltac:(lia)). destruct AFTER as [NEQ AFTER].
-      split; [congruence| ].
+      split; [congruence| ]. 
       intros.
       assert (k <= i \/ i <= k <= i + m) as [BEFORE | CUR] by lia. 
-      2: { intros [? LOCK2].
+      2: {
+           intros [LOCK2 DIS2].
            specialize (BETWEEN (k - i)). specialize_full BETWEEN.
            { lia. }
            { erewrite state_lookup_after; eauto.
              rewrite -Nat.le_add_sub; eauto. lia. }
-           apply proj1 in BETWEEN. simpl in LOCK2.
-           eapply NEQ. eapply has_lock_st_excl; eauto. }
+
+           simpl in LOCK2. destruct LOCK2 as [DOM [LOCK2 | ?]]. 
+           2: { red in DIS2. tauto. }
+           destruct LOCK2 as [? [EN | ?]]. 
+           { by apply ls_mapping_dom, enabled_group_singleton in EN. }
+           eapply NEQ. eapply (has_lock_st_excl st_k (FairLock := FL)); eauto.
+           all: try tauto.
+           by apply disabled_group_disabled_role. }
       
       move PREi at bottom. red in PREi.
       setoid_rewrite pred_at_trace_lookup in PREi. specialize_full PREi.
@@ -564,30 +924,43 @@ Section FairLockLM.
       { eexists. eauto. }
       destruct PREi as (p & (st&PTH&->) & LT').
       apply AFTER in PTH; [| lia].
-      set_solver. }
+      intros [LOCK DIS]. apply PTH.
+      split.
+      2: { eapply disabled_group_disabled_role; eauto. }
+      simpl in LOCK. destruct LOCK as [? [? | ?]].
+      2: { red in DIS. tauto. }
+      tauto. }
+    { done. }
+
+    intros ER. 
+    destruct ER as (p & δ_p & ? & ? & PTH).
+        
+    (* pose proof PTH as PTH_.  *)
     
-    destruct EV_REL as (p & δ_p & PTH & LEm & ENp).
-    assert (i <= p) as [d ->]%Nat.le_sum by lia. 
-    erewrite <-state_lookup_after in PTH; eauto.
-    eapply upto_stutter_state_lookup' in PTH as [c CTH]; eauto.
-    exists (j + c). eexists. repeat split.
-    { erewrite <- state_lookup_after; eauto. }
+    assert (i <= p) as [d ->]%Nat.le_sum by lia.
+    erewrite <- @trace_lookup_after in PTH; eauto.
+
+    eapply upto_stutter_trace_label_lookup in PTH; eauto.
+    simpl in PTH. destruct PTH as [c CTH].
+    apply trace_label_lookup_simpl' in CTH as (?&?&CTH).
+    erewrite trace_lookup_after in CTH; eauto.
+    exists (j + c + 1). eexists. repeat split.
+    { apply state_label_lookup in CTH as (?&?&?). eauto. }
     { lia. }
-    apply ENp.
+    eapply trace_valid_steps' in CTH; eauto.
+    2: { eapply destutter_ext.upto_preserves_validity; eauto.
+         apply PROJ_KEEP_EXT. }
+    inversion CTH; subst. simpl in REL.
+    apply au_impl_spec in REL. apply REL. 
   Qed. 
 
-  Instance oob_dec: forall ρ δ1 ℓ δ2, Decision (others_or_burn ρ δ1 ℓ δ2). 
-  Proof. 
-    rewrite /others_or_burn. destruct ℓ as [[|]|]; apply _. 
-  Qed. 
-
-  Instance oob_lookup_dec: ∀ x (lmtr: elmftrace (ELM := FL_EM FLE_LMF)) ρ,
+  Instance oob_lookup_dec: ∀ x (lmtr: elmftrace (ELM := FL_EM FLE_LMF)) ρ flc,
     Decision
       (∃ (δ1 : LiveState G M LSI) (ℓ : option (G + env_role)) 
          (δ2 : LiveState G M LSI),
-         lmtr !! x = Some (δ1, Some (ℓ, δ2)) ∧ ¬ others_or_burn ρ δ1 ℓ δ2).
+         lmtr !! x = Some (δ1, Some (ℓ, δ2)) ∧ ¬ others_or_burn ρ flc δ1 ℓ δ2).
   Proof. 
-    intros k lmtr ρ. destruct (lmtr !! k) as [[? [[ℓ ?]|]] | ] eqn:K.
+    intros k lmtr ρ flc. destruct (lmtr !! k) as [[? [[ℓ ?]|]] | ] eqn:K.
     2, 3: right; set_solver.
     eapply Decision_iff_impl.
     { erewrite ex_det_iff3.
@@ -596,8 +969,8 @@ Section FairLockLM.
     solve_decision. 
   Qed. 
 
-  Lemma final_steps ρ i (P: R → fmstate M → Prop)
-    (lmtr: mtrace (@ext_model_FM LMF (@FL_EM LMF FLE_LMF)))
+  Lemma final_steps ρ i (P P': R → fmstate M → Prop) flc
+    (lmtr: mtrace (@ext_model_FM LMF (@FL_EM LMF _ FLE_LMF)))
     (δ : LiveState G M LSI)
     (DISM : fair_lock.disabled_st ρ (ls_under δ))
     (* (LOCK : has_lock_st ρ (ls_under δ)) *)
@@ -606,20 +979,24 @@ Section FairLockLM.
     (USED: forall ρ st, P ρ st -> ¬ is_unused ρ st)
     (KEPT: forall ρ, label_kept_state_gen
              (λ st : fmstate (@ext_model_FM _ (FL_EM FLE_LMF)),
-                 P ρ (ls_under st) ∧ fair_lock.disabled_st ρ (ls_under st)) (others_or_burn ρ))
+                 P ρ (ls_under st) ∧ fair_lock.disabled_st ρ (ls_under st)) (others_or_burn ρ flc))
     (FAIR: ∀ g, fair_by_group (ELM_ALM LM_EM_EXT_KEEPS) g lmtr)
-    (VALID: mtrace_valid lmtr):
+    (VALID: mtrace_valid lmtr)
+    (FLC_PROJ: forall (g: fmrole LMF), proj_role (inr $ env $ flc g) = g)
+    :
     ∃ (n : nat) (st' : fmstate ext_model_FM),
       i <= n
       ∧ lmtr S!! n = Some st'
-      ∧ lift_prop1 P (asG ρ) st' ∧ fair_lock.disabled_st (asG ρ) st'.
+      ∧ lift_prop1 P P' (asG ρ) st' ∧ fair_lock.disabled_st (asG ρ) st'.
   Proof.
     destruct (decide (ρ ∈ dom (ls_mapping δ))) as [MAP | UNMAP]. 
     2: { eapply unmapped_empty in UNMAP.
          2: { eauto. }
          exists i, δ. split; [lia| ].
          repeat split; try done. 
-         all: eapply elem_of_dom; eauto. }
+         { eapply elem_of_dom; eauto. }
+         { left. split; auto. right. apply LM_map_empty_notlive. by left. }
+         apply LM_map_empty_notlive. by left. }
 
     apply group_fairness_implies_step_or_unassign with (ρ := ρ) in FAIR; [| done].
     apply fair_by_gen_equiv, fair_by_gen'_strong_equiv in FAIR. 
@@ -631,7 +1008,7 @@ Section FairLockLM.
     destruct FAIR as (p & δ' & step' & PTH & STEPp & MINp).
     rewrite /fairness_sat_gen in MINp. 
 
-    edestruct (list_exist_dec (fun m => exists δ1 ℓ δ2, lmtr !! m = Some (δ1, Some (ℓ, δ2)) /\ ¬ others_or_burn ρ δ1 ℓ δ2) (seq i p)) as [EXT | NOEXT].
+    edestruct (list_exist_dec (fun m => exists δ1 ℓ δ2, lmtr !! m = Some (δ1, Some (ℓ, δ2)) /\ ¬ others_or_burn ρ flc δ1 ℓ δ2) (seq i p)) as [EXT | NOEXT].
     { solve_decision. }
     - destruct EXT as [k_ EXT].
       pattern k_ in EXT. eapply min_prop_dec in EXT as [k [EXT MINk]]; [clear k_|].
@@ -645,48 +1022,59 @@ Section FairLockLM.
       { auto. }
       3: { eapply trace_state_lookup. apply KTH. }
       2: { split; [| reflexivity]. lia. }
-      { intros. destruct (decide (others_or_burn ρ st1 oℓ' st2)); [done| ].
+      { intros. destruct (decide (others_or_burn ρ flc st1 oℓ' st2)); [done| ].
         specialize (MINk k0). specialize_full MINk; [| lia].
         split; eauto.
         apply elem_of_seq. lia. }
-      intros [LOCKk DISk]. 
+      intros [LOCKk DISk].
+
+      assert (ls_tmap x !! asG ρ = Some ∅).
+      { 
+
+        rewrite /others_or_burn in STEP. destruct ℓ as [r| ].
+        2: { simpl in STEP. tauto. }
+        destruct r.
+        { apply NNP_P in STEP.
+          edestruct disabled_not_live; eauto. 
+          apply next_TS_spec_pos in STEP. eapply fm_live_spec.
+          apply STEP. }
+        destruct e. 
+        simpl in STEP. apply NNP_P in STEP. 
+        eapply trace_valid_steps' in KTH; eauto. inversion KTH.
+        revert STEP. subst. intros STEP.
+        pose proof (FLC_PROJ (asG ρ)). simpl in H. rewrite -STEP in H. 
+        destruct i0; subst; simpl in REL.
+        - apply REL.
+        - apply REL. }
 
       exists k. eexists. repeat split. 
       { lia. }        
       { eapply trace_state_lookup; eauto. }
       { apply not_unused_dom. eauto. }
-      all: auto. 
-      2: { apply not_unused_dom. eauto. }
-      
-      rewrite /others_or_burn in STEP. destruct ℓ as [r| ].
-      2: { simpl in STEP. tauto. }
-      destruct r.
-      { apply NNP_P in STEP.
-        edestruct disabled_not_live; eauto. 
-        apply next_TS_spec_pos in STEP. eapply fm_live_spec.
-        apply STEP. }
-      simpl in STEP. apply NNP_P in STEP.
-      eapply trace_valid_steps' in KTH; eauto. inversion KTH; subst.
-      destruct ι; subst; simpl in REL.
-      1, 2: apply proj1 in REL; by rewrite REL. 
+      all: auto.
+      { left. split; auto. right. apply LM_map_empty_notlive. by left. }
+      apply LM_map_empty_notlive. by left.       
     - forward eapply steps_keep_state_gen.
       3: { apply KEPT. }
       2: { eexists. split; [eapply DTH| ]. eauto. }
       { eauto. }
       3: { eapply trace_state_lookup. apply PTH. }
       2: { split; [lia| ]. reflexivity. }
-      { intros. destruct (decide (others_or_burn ρ st1 oℓ' st2)); [done| ].
+      { intros. destruct (decide (others_or_burn ρ flc st1 oℓ' st2)); [done| ].
         edestruct NOEXT. exists k. split; eauto. 
         apply elem_of_seq. lia. }
       intros [LOCKp DISp].
 
       red in STEPp. destruct STEPp as [UNMAP | STEP]. 
-      + do 2 eexists. repeat split.
+      +
+        assert (¬ role_enabled_model ((asG ρ): fmrole LMF) δ').
+        { apply LM_map_empty_notlive. left.
+          eapply unmapped_empty; eauto. }
+        do 2 eexists. repeat split.
         2: { eapply trace_state_lookup, PTH. }
         { lia. }
         all: eauto.
-        1, 3: apply not_unused_dom; by eauto. 
-        eapply unmapped_empty; eauto.
+        1: apply not_unused_dom; by eauto.
       + red in STEP. destruct STEP as (?&?&?&[=]&<-&STEP); subst.
         apply next_TS_spec_pos in STEP.
         eapply disabled_not_live in DISp. destruct DISp.
@@ -698,6 +1086,35 @@ Section FairLockLM.
     @fl_lock_progress _ FLP_LMF (FL_EM FLE_LMF) (fun tr => forall g, fair_by_group (ELM_ALM LM_EM_EXT_KEEPS) g tr). 
   Proof.
     red. intros lmtr [ρ] i δ **.
+   
+    simpl in CAN_LOCK. destruct CAN_LOCK as [DOM [L | U]].
+    2: { pose proof (group_fairness_implies_step_or_unassign _ _ VALID FAIR) as FAIR'.
+         specialize (FAIR' ρ). red in FAIR'.
+         apply fair_by_gen_equiv, fair_by_gen'_strong_equiv in FAIR'.
+         2, 3: solve_decision. 
+         specialize (FAIR' i). specialize_full FAIR'.
+         { rewrite ITH. simpl.
+           do 2 red in ACT. apply LM_live_roles_strong in ACT as [? STEP]. 
+           apply locale_trans_ex_role in STEP as [ρ_ IN].
+           pose proof IN as EQ%MAP_RESTR.
+           eapply elem_of_dom. set_solver. }
+
+         forward eapply final_steps with (P := does_unlock) (P' := does_lock).
+         { apply U. }
+         { apply U. }
+         { apply ITH. }
+         { intros. intros ?. eapply unused_does_unlock_incompat; eauto. }
+         { apply others_or_burn_keep_lock. }
+         { done. }
+         { done. }
+         { done. }
+         intros (n&?&?&?&?&?). exists n. eexists. split; [| eauto].
+         apply Nat.le_lteq in H as [? | ->]; [done| ].
+         congruence. }
+
+    destruct L as [L [EN | DIS]].
+    2: { by red in ACT. } 
+
     pose proof (group_fairness_implies_role_fairness _ _ VALID FAIR) as FAIR'.
     pose proof (can_destutter_eauxtr proj_ext _ VALID) as [mtr UPTO].
     forward eapply destutter_ext.upto_preserves_validity as VALIDm; eauto. 
@@ -714,8 +1131,6 @@ Section FairLockLM.
     { eapply trace_valid_after; eauto. }
     { do 2 red. intros. eapply fair_by_after; eauto. by apply FAIRm. }
     { erewrite state_lookup_after; eauto. by rewrite Nat.add_0_r. }
-    { apply CAN_LOCK. }
-    { apply ACT. }
     { eapply ev_rel_after in EV_REL; eauto.
       eapply ev_rel_inner; eauto.
       - eapply trace_valid_after; eauto. 
@@ -729,14 +1144,14 @@ Section FairLockLM.
     assert (d > 0) as NZd.
     { destruct d; [| lia].
       rewrite Nat.add_0_r ITH in DTH. inversion DTH. subst δ'.
-      simpl in CAN_LOCK.
-      edestruct can_has_lock_incompat; eauto.
-      apply CAN_LOCK. }  
+      edestruct does_lock_unlock_incompat; eauto. } 
     
-    forward eapply final_steps; eauto.
-    { intros ** ?. eapply unused_has_lock_incompat; eauto. }
+    forward eapply final_steps with (P' := does_lock); eauto.
+    { intros ** ?. eapply unused_does_unlock_incompat; eauto. }
     { apply others_or_burn_keep_lock. }
-    intros (n&?&?&?&?&?). exists n. eexists. split; [| eauto]. lia. 
+    { done. }
+    intros (n&?&?&?&?&?). exists n. eexists. split; [| eauto].
+    lia. 
   Qed.
 
   Lemma FL_LM_unlock:
@@ -744,6 +1159,35 @@ Section FairLockLM.
   Proof.
     red. intros lmtr [ρ] i δ **.
     rename CAN_LOCK into LOCK. 
+
+    simpl in LOCK. destruct LOCK as [DOM [L | U]].
+    2: { pose proof (group_fairness_implies_step_or_unassign _ _ VALID FAIR) as FAIR'.
+         specialize (FAIR' ρ). red in FAIR'.
+         apply fair_by_gen_equiv, fair_by_gen'_strong_equiv in FAIR'.
+         2, 3: solve_decision. 
+         specialize (FAIR' i). specialize_full FAIR'.
+         { rewrite ITH. simpl.
+           do 2 red in ACT. apply LM_live_roles_strong in ACT as [? STEP]. 
+           apply locale_trans_ex_role in STEP as [ρ_ IN].
+           pose proof IN as EQ%MAP_RESTR.
+           eapply elem_of_dom. set_solver. }
+
+         forward eapply final_steps with (P := does_lock) (P' := does_unlock).
+         { apply U. }
+         { apply U. }
+         { apply ITH. }
+         { intros. intros ?. eapply unused_does_lock_incompat; eauto. }
+         { apply others_or_burn_keep_can_lock. }
+         { done. }
+         { done. }
+         { done. }
+         intros (n&?&?&?&?&?). exists n. eexists. split; [| eauto].
+         apply Nat.le_lteq in H as [? | ->]; [done| ].
+         congruence. }
+
+    destruct L as [L [EN | DIS]].
+    2: { by red in ACT. } 
+
     pose proof (group_fairness_implies_role_fairness _ _ VALID FAIR) as FAIR'.
     pose proof (can_destutter_eauxtr proj_ext _ VALID) as [mtr UPTO].
     forward eapply destutter_ext.upto_preserves_validity as VALIDm; eauto. 
@@ -760,8 +1204,6 @@ Section FairLockLM.
     { eapply trace_valid_after; eauto. }
     { do 2 red. intros. eapply fair_by_after; eauto. by apply FAIRm. }
     { erewrite state_lookup_after; eauto. by rewrite Nat.add_0_r. }
-    { apply LOCK. }
-    { apply ACT. }
     
     destruct PROGRESSm as (d' & st & NZ & DTH' & UNLOCK & DISM).
     eapply upto_stutter_state_lookup in DTH' as (d & δ' & DTH & CORRd); [| by apply UPTOi].
@@ -771,241 +1213,36 @@ Section FairLockLM.
     assert (d > 0) as NZd.
     { destruct d; [| lia].
       rewrite Nat.add_0_r ITH in DTH. inversion DTH. subst δ'.
-      edestruct can_has_lock_incompat; eauto.
-      apply LOCK. }
+      edestruct does_lock_unlock_incompat; eauto. }
     clear dependent δ. rename δ' into δ. 
 
-    forward eapply final_steps; eauto.
-    { intros ** ?. eapply unused_can_lock_incompat; eauto. }
+    forward eapply final_steps with (P' := does_unlock); eauto.
+    { intros ** ?. eapply unused_does_lock_incompat; eauto. }
     { apply others_or_burn_keep_can_lock. }
+    { done. }
     intros (n&?&?&?&?&?). exists n. eexists. split; [| eauto]. lia. 
-  Qed.     
-
-  Lemma FL_LM_term:
-    @fl_trace_termination _ FLP_LMF (FL_EM FLE_LMF) (fun tr => forall g, fair_by_group (ELM_ALM LM_EM_EXT_KEEPS) g tr). 
-  Proof.
-    red. intros lmtr **. 
-    pose proof (group_fairness_implies_role_fairness _ _ VALID FAIR) as FAIR'.
-    pose proof (can_destutter_eauxtr proj_ext _ VALID) as [mtr UPTO].
-    forward eapply destutter_ext.upto_preserves_validity as VALIDm; eauto. 
-    { apply PROJ_KEEP_EXT. }
-    forward eapply destutter_ext.upto_stutter_fairness as FAIRm; eauto.
-    { eapply ELM_ALM_afair_by_next; eauto. }
-
-    eapply destutter_ext.upto_stutter_finiteness; eauto.
-    apply trace_termination; eauto.
-    { eapply ext_bounded_inner; eauto. }
-    intros.
-
-    red. intros.
-
-    forward eapply upto_state_lookup_unfold1 as (mtr_i' & i' & lmtr_i & AFTERi & AFTERi' & UPTOi & ITH' & ?); eauto. 
-
-    forward eapply disable_lmtr as D; eauto.
-    destruct D as (m & δ_m & LEi & MTH & HAS_LOCK' & UNMAP & BETWEEN).
-
-    assert (ls_tmap δ_m !! asG ρ' = Some ∅) as DOMρ'.
-    { apply unmapped_empty; auto. intros UN. 
-      edestruct unused_has_lock_incompat; eauto. } 
-
-    move EV_REL at bottom.
-    specialize (EV_REL (asG ρ) (S m)). red in EV_REL. specialize_full EV_REL; eauto.
-    { Unshelve. 2: exact (asG ρ'). simpl. split; auto.
-      eapply elem_of_dom; eauto. }
-    { split; eauto. 
-      red. split; [by eapply elem_of_dom| ]. 
-      eapply (BETWEEN (m - i')).
-      { lia. }
-      erewrite state_lookup_after; eauto.
-      rewrite -Nat.le_add_sub; eauto. } 
-    { lia. }
-
-    destruct EV_REL as (p & δ_p & PTH & LEm & ENp).
-    assert (i' <= p) as [d ->]%Nat.le_sum by lia. 
-    erewrite <-state_lookup_after in PTH; eauto.
-    eapply upto_stutter_state_lookup' in PTH as [c CTH]; eauto.
-    exists (j + c). eexists. repeat split.
-    { erewrite <- state_lookup_after; eauto. }
-    { lia. }
-    apply ENp.
   Qed.
-
 
   (* TODO: is it possible to avoid delegating this to user? *)
   Context {allow_unlock_impl: G -> lm_ls LM -> lm_ls LM}.
-  Hypothesis (allows_unlock_impl_spec: forall g δ δ', allows_unlock g δ δ' <->
-             (allow_unlock_impl g δ = δ' /\ (has_lock_st g δ /\ disabled_st g δ))).
+  Hypothesis (allows_unlock_impl_spec: forall g δ δ', au_impl g δ δ' <->
+             (allow_unlock_impl g δ = δ' /\ (does_unlock g δ /\ disabled_st g δ))).
   Hypothesis (allow_unlock_post: forall g δ, 
-                 has_lock_st g δ /\ disabled_st g δ ->
+                 does_unlock g δ /\ disabled_st g δ ->
                  let δ' := allow_unlock_impl g δ in
-                 has_lock_st g δ' /\ active_st g δ'). 
+                 does_unlock g δ' /\ active_st g δ'). 
 
   Context {allow_lock_impl: G -> lm_ls LM -> lm_ls LM}.
-  Hypothesis (allows_lock_impl_spec: forall g δ δ', allows_lock g δ δ' <->
-             (allow_lock_impl g δ = δ' /\ (can_lock_st g δ /\ disabled_st g δ))).
+  Hypothesis (allows_lock_impl_spec: forall g δ δ', al_impl g δ δ' <->
+             (allow_lock_impl g δ = δ' /\ (does_lock g δ /\ disabled_st g δ))).
 
-
-  (* TODO: refactor *)
-  Lemma can_lock_dis_kept:
-    ∀ ρ : fmrole LMF,
-    @label_kept_state (@ext_model_FM LMF (@FL_EM LMF FLE_LMF))
-      (λ st : fmstate (@ext_model_FM LMF (@FL_EM LMF FLE_LMF)),
-         @can_lock_st LMF FLP_LMF ρ st ∧ @fair_lock.disabled_st LMF FLP_LMF ρ st)
-      (@other_proj LMF FLE_LMF ρ).
-  Proof.
-    red. intros [ρ] δ oℓ δ' [LOCK DIS] OTHER STEP.
-    simpl in STEP. 
-    inversion STEP; subst.
-    - assert (can_lock_st ρ (ls_under δ') /\ fair_lock.disabled_st ρ (ls_under δ') /\ ls_tmap δ' !! asG ρ = Some ∅) as (?&?&?).
-      { simpl in STEP0, LOCK, DIS.
-        simpl in OTHER.  destruct ρ0 as [ρ'].
-
-       assert (ρ ∉ dom (ls_mapping δ)) as ND. 
-       { intros IN.
-         apply elem_of_dom in IN as [? MAP].
-         pose proof MAP as ->%MAP_RESTR.
-         apply proj1 in DIS.
-         apply ls_mapping_tmap_corr in MAP as (?&?&?).
-         rewrite DIS in H. set_solver. }
-        
-        unfold_LMF_trans STEP0.
-        2: { simpl in STEP1. pose proof STEP1 as SS. repeat apply proj2 in STEP1.
-            rewrite -STEP1. repeat split; try tauto.
-            apply unmapped_empty.
-            { intros ?. rewrite STEP1 in LOCK.
-              edestruct unused_can_lock_incompat; eauto. apply LOCK. }
-            intros IN. 
-            pose proof SS.
-            do 3 apply proj2 in SS. apply proj1 in SS.
-            repeat rewrite -ls_same_doms in SS.
-            set_solver. }
-        forward eapply (step_keeps_can_lock_dis ρ (ls_under δ)).
-        { split; [apply LOCK | apply DIS]. }
-        2: { left. apply STEP1. }
-        { simpl. intros ->.
-          apply proj1 in DIS.
-          simpl in STEP1. apply proj2, proj1 in STEP1.
-          pose proof STEP1 as (?&?&?)%ls_mapping_tmap_corr.
-          by apply MAP_RESTR in STEP1. }
-        intros [??]. repeat split; eauto.
-        simpl in STEP1.
-        apply unmapped_empty.
-        { intros ?. edestruct unused_can_lock_incompat; eauto. }
-        intros IN.
-        repeat apply proj2 in STEP1. specialize (STEP1 ρ). specialize_full STEP1.
-        { apply elem_of_difference. repeat rewrite -ls_same_doms. split; [done| ].
-          intros IN'. done. }
-        apply elem_of_difference, proj1 in STEP1.
-        eapply disabled_not_live in H0; eauto. }
-      
-      simpl. repeat split; eauto.
-      all: by apply elem_of_dom. 
-    - forward eapply (step_keeps_can_lock_dis ρ δ) as KEPT. 
-      { split; [apply LOCK| apply DIS]. }
-      2: { right. eapply PROJ_KEEP_EXT; eauto. }
-      { simpl. simpl in OTHER.
-        destruct ι; simpl; simpl in OTHER; red; destruct ρ0; congruence. }
-      intros. 
-      destruct ι; simpl in REL; red in REL.
-      + destruct ρ0 as [ρ']. assert (ρ' ≠ ρ) by set_solver. 
-        simpl in *.
-        enough (ls_tmap δ' !! asG ρ = Some ∅).
-        { repeat split; eauto; try by apply KEPT.
-          all: eapply elem_of_dom; eauto. }
-        apply proj2, proj1 in REL. rewrite REL.
-        rewrite lookup_insert_ne; [| done]. tauto. 
-      + destruct ρ0 as [ρ']. assert (ρ' ≠ ρ) by set_solver. 
-        simpl in *.
-        enough (ls_tmap δ' !! asG ρ = Some ∅).
-        { repeat split; eauto; try by apply KEPT.
-          all: eapply elem_of_dom; eauto. }
-        apply proj2, proj1 in REL. rewrite REL.
-        rewrite lookup_insert_ne; [| done]. tauto. 
-  Qed.  
-    
-  Lemma lock_dis_kept:
-    ∀ ρ : fmrole LMF,
-    @label_kept_state (@ext_model_FM LMF (@FL_EM LMF FLE_LMF))
-      (λ st : fmstate (@ext_model_FM LMF (@FL_EM LMF FLE_LMF)),
-         @has_lock_st LMF FLP_LMF ρ st ∧ @fair_lock.disabled_st LMF FLP_LMF ρ st)
-      (@other_proj LMF FLE_LMF ρ).
-  Proof.
-    red. intros [ρ] δ oℓ δ' [LOCK DIS] OTHER STEP.
-    simpl in STEP. 
-    inversion STEP; subst.
-    - assert (has_lock_st ρ (ls_under δ') /\ fair_lock.disabled_st ρ (ls_under δ') /\ ls_tmap δ' !! asG ρ = Some ∅) as (?&?&?).
-      { simpl in STEP0, LOCK, DIS.
-        simpl in OTHER.  destruct ρ0 as [ρ'].
-
-       assert (ρ ∉ dom (ls_mapping δ)) as ND. 
-       { intros IN.
-         apply elem_of_dom in IN as [? MAP].
-         pose proof MAP as ->%MAP_RESTR.
-         apply proj1 in DIS.
-         apply ls_mapping_tmap_corr in MAP as (?&?&?).
-         rewrite DIS in H. set_solver. }
-        
-        unfold_LMF_trans STEP0.
-        2: { simpl in STEP1. pose proof STEP1 as SS. repeat apply proj2 in STEP1.
-            rewrite -STEP1. repeat split; try tauto.
-            apply unmapped_empty.
-            { intros ?. rewrite STEP1 in LOCK.
-              edestruct unused_has_lock_incompat; eauto. apply LOCK. }
-            intros IN. 
-            pose proof SS.
-            do 3 apply proj2 in SS. apply proj1 in SS.
-            repeat rewrite -ls_same_doms in SS.
-            set_solver. }
-        forward eapply (step_keeps_lock_dis ρ (ls_under δ)).
-        { split; [apply LOCK | apply DIS]. }
-        2: { left. apply STEP1. }
-        { simpl. intros ->.
-          apply proj1 in DIS.
-          simpl in STEP1. apply proj2, proj1 in STEP1.
-          pose proof STEP1 as (?&?&?)%ls_mapping_tmap_corr.
-          by apply MAP_RESTR in STEP1. }
-        intros [??]. repeat split; eauto.
-        simpl in STEP1.
-        apply unmapped_empty.
-        { intros ?. edestruct unused_has_lock_incompat; eauto. }
-        intros IN.
-        repeat apply proj2 in STEP1. specialize (STEP1 ρ). specialize_full STEP1.
-        { apply elem_of_difference. repeat rewrite -ls_same_doms. split; [done| ].
-          intros IN'. done. }
-        apply elem_of_difference, proj1 in STEP1.
-        eapply disabled_not_live in H0; eauto. }
-      
-      simpl. repeat split; eauto.
-      all: by apply elem_of_dom. 
-    - forward eapply (step_keeps_lock_dis ρ δ) as KEPT. 
-      { split; [apply LOCK| apply DIS]. }
-      2: { right. eapply PROJ_KEEP_EXT; eauto. }
-      { simpl. simpl in OTHER.
-        destruct ι; simpl; simpl in OTHER; red; destruct ρ0; congruence. }
-      intros. 
-      destruct ι; simpl in REL; red in REL.
-      + destruct ρ0 as [ρ']. assert (ρ' ≠ ρ) by set_solver. 
-        simpl in *.
-        enough (ls_tmap δ' !! asG ρ = Some ∅).
-        { repeat split; eauto; try by apply KEPT.
-          all: eapply elem_of_dom; eauto. }
-        apply proj2, proj1 in REL. rewrite REL.
-        rewrite lookup_insert_ne; [| done]. tauto. 
-      + destruct ρ0 as [ρ']. assert (ρ' ≠ ρ) by set_solver. 
-        simpl in *.
-        enough (ls_tmap δ' !! asG ρ = Some ∅).
-        { repeat split; eauto; try by apply KEPT.
-          all: eapply elem_of_dom; eauto. }
-        apply proj2, proj1 in REL. rewrite REL.
-        rewrite lookup_insert_ne; [| done]. tauto. 
-  Qed.  
     
   Lemma unused_kept_LM:
   ∀ ρ : fmrole LMF,
-    @label_kept_state (@ext_model_FM LMF (@FL_EM LMF FLE_LMF))
-      (λ st : fmstate (@ext_model_FM LMF (@FL_EM LMF FLE_LMF)),
+    @label_kept_state (@ext_model_FM LMF (@FL_EM LMF _ FLE_LMF))
+      (λ st : fmstate (@ext_model_FM LMF (@FL_EM LMF _ FLE_LMF)),
          @is_unused LMF FLP_LMF ρ st)
-      (λ _ : option (fmrole (@ext_model_FM LMF (@FL_EM LMF FLE_LMF))), True).
+      (λ _ : option (fmrole (@ext_model_FM LMF (@FL_EM LMF _ FLE_LMF))), True).
   Proof.
     intros [ρ] δ oℓ δ' UNUSED _ STEP.
     inversion STEP; subst.
@@ -1029,29 +1266,33 @@ Section FairLockLM.
       fair_lock.allow_unlock_impl := allow_unlock_impl;
       fair_lock.allow_lock_impl := allow_lock_impl;
     |}. 
-  16: { apply FL_LM_term. }
-  15: { apply FL_LM_unlock. }
-  14: { apply FL_LM_progress. }
-  - simpl. 
-    apply allows_unlock_impl_spec. 
+  (* 16: { apply FL_LM_term. } *)
+  14: { apply FL_LM_unlock. }
+  13: { apply FL_LM_progress. }
+  - simpl. apply allows_unlock_impl_spec. 
   - simpl. apply allows_lock_impl_spec.
-  - apply lock_dis_kept.
-  - apply can_lock_dis_kept. 
+  - apply does_unlock_dis_kept. 
+  - apply does_lock_dis_kept.
   - apply unused_kept_LM.
   - intros ? []. simpl. tauto.
   - intros ? []. simpl. tauto.
-  - intros ? []. simpl. tauto.
-  - intros ? []. simpl. tauto.
-  - intros ? []. simpl. intros (EMP&_).
-    apply LM_map_empty_notlive. tauto.
-  - intros ? [ρ1] [ρ2]. simpl.
-    intros [??] [??]. f_equal.
-    eapply has_lock_st_excl; eauto.
+  - intros ? []. simpl. intros ? (?&?&?)%LM_live_role_map_notempty.
+    destruct H. by apply elem_of_dom. 
+  - done. 
+  - apply has_lock_excl_lift. 
   - intros ? []. simpl.
-    intros [??] [??]. eapply can_has_lock_incompat; eauto.
-  - intros ? [ρ] ?. intros (<-&?&?)%allows_unlock_impl_spec.
-    apply and_assoc. split; [done| ]. 
-    eapply allow_unlock_post. eauto. 
+    intros [? R1] [? R2].
+    destruct R1, R2.
+    2, 3: tauto. 
+    { eapply does_lock_unlock_incompat; [apply H1| apply H2]. }
+    { eapply does_lock_unlock_incompat; [apply H2| apply H1]. }
+  - intros δ [ρ]. simpl.
+    destruct (decide (asG ρ ∈ dom (ls_tmap δ))); [| tauto].
+    apply or_assoc. left.
+    pose proof (fair_lock.does_lock_unlock_trichotomy (ls_under δ) ρ) as T.
+    apply or_assoc in T as [T | U].
+    2: { by apply UNUSED_NOT_DOM in U. }
+    destruct (decide (role_enabled_model ρ (ls_under δ))), (decide (role_enabled_model ((asG ρ): fmrole LMF) δ)); tauto.
   Qed. 
 
 End FairLockLM.
